Aesop/Search/Expansion/Test.lean
@@ -1,0 +1,51 @@
+import Aesop.Search.Expansion.Norm
+import Lean.Meta
+open Lean Meta
+--NVU
+/-
+def setupGoal : IO MVarId := do
+  let goalType := mkConst`Nat
+  let goalExpr ← mkFreshExprMVar goalType
+  return goalExpr.mvarId
+
+def testReduceAllInGoal : MetaM Bool := do
+  let goal ← setupGoal
+  let originalType ← goal.getType
+  let reducedGoal ← reduceAllInGoal goal
+  let newType ← reducedGoal.getType
+  return originalType ≠ newType
+
+def runTest : IO Unit := do
+  let env ← MetaM.run testReduceAllInGoal
+  if env then
+    IO.println "Test passed: Goal was reduced."
+  else
+    IO.println "Test failed: Goal was not reduced."
+-/
+
+abbrev Foo := Nat
+
+run_meta show MetaM Unit from do
+  let goal ← Lean.Meta.mkFreshExprMVar (mkConst `Nat)
+  logInfo m!"Generated goal: {goal}"
+
+example : Foo := by
+  run_tac do
+    let e <- Elab.Tactic.getMainTarget
+    let e' <- reduceAll e
+    logInfo e'
+  exact 1
+
+
+abbrev Bopo := Nat
+
+run_meta show MetaM Unit from do
+  let goal ← Lean.Meta.mkFreshExprMVar (mkConst `Bool)
+  logInfo m!"Generated goal: {goal}"
+
+example : Bopo := by
+  run_tac do
+    let e <- Elab.Tactic.getMainTarget
+    let e' <- reduceAll e
+    logInfo e'
+  exact 5
